Les robots adpatés à la nouvelle version des multisets

gathering-nD/MMultiset/MMultisetMap.v
@@ -9,7 +9,7 @@
 (******************************************)
 
 
-Require Import FMapInterface.
+Require Import MMapInterface.
 Require Import Arith_base.
 Require Import Omega.
 Require Import PArith.
@@ -18,19 +18,13 @@ Require Import MMultiset.Preliminary.
 Require Import MMultisetInterface.
 Require Import Equalities.
 
-Module FMultisets (FMap : WSfun) (E : DecidableType.DecidableType) : FMultisetsOn E.
+Module FMultisets (MMap : WSfun) (E : DecidableType) : FMultisetsOn E.
 
-Module M := FMap(E).
+Module M := MMap(E).
 
 Definition eq_pair := RelProd E.eq (@Logic.eq nat).
 Definition eq_key := RelCompFun E.eq (@fst E.t nat).
 
-Instance Eeq_equiv : Equivalence E.eq.
-Proof. split.
-  exact E.eq_refl.
-  exact E.eq_sym.
-  exact E.eq_trans.
-Qed.
 
 Instance Meq_equiv A : Equivalence (@M.eq_key_elt A).
 Proof. split.
@@ -75,19 +69,26 @@ intros A x y n m l Hl Hinx Hiny Heq. induction Hl as [| [z p] l]. inversion_clea
 inversion_clear Hinx; inversion_clear Hiny.
 - compute in H0, H1. destruct H0 as [H0 ?], H1 as [H1 ?]. now subst p m.
 - compute in H0. destruct H0 as [H0 ?]. subst p. elim H.
-  apply eq_key_elt_eq_key_weak_In with y m. transitivity x; auto. assumption.
+  apply eq_key_elt_eq_key_weak_In with y m. now transitivity x. assumption.
 - compute in H1. destruct H1 as [H1 ?]. subst p. elim H.
   apply eq_key_elt_eq_key_weak_In with x n. now transitivity y; auto. assumption.
 - now apply IHHl.
 Qed.
 
-Lemma Melements_InA : forall A x n s, InA (@M.eq_key_elt A) (x, n) (M.elements s) <-> M.MapsTo x n s.
-Proof. intros. split; intro H. now apply M.elements_2. now apply M.elements_1. Qed.
+Lemma Melements_InA : forall A x n s, InA (@M.eq_key_elt A) (x, n) (M.bindings s) <-> M.MapsTo x n s.
+Proof. intros. now apply M.bindings_spec1. Qed.
+
+Instance Mfind_compat {A} : Proper (E.eq ==> @M.Equal A ==> Logic.eq) (@M.find A).
+Proof.
+intros x1 x2 Hx s1 s2 Hs. rewrite Hs. clear s1 Hs. destruct (M.find x1 s2) eqn:Hin.
+- rewrite M.find_spec, Hx, <- M.find_spec in Hin. auto.
+- destruct (M.find x2 s2) eqn:Hin'; trivial. rewrite M.find_spec, <- Hx, <- M.find_spec, Hin in Hin'. discriminate.
+Qed.
 
 Definition elt := E.t.
 Definition t := M.t positive.
 
-Definition empty : t := M.empty positive.
+Definition empty : t := @M.empty positive.
 Definition is_empty (s : t) := M.is_empty s.
 Definition multiplicity x (s : t) := match M.find x s with Some n => Pos.to_nat n | None => 0 end.
 Definition add (x : elt) (n : nat) (s : t) : t := 
@@ -103,7 +104,6 @@ Definition diff (s s' : t) := M.fold (fun x n acc => add x (Pos.to_nat n - multi
 Definition lub (s s' : t) := M.fold (fun x n acc => add x (Pos.to_nat n - multiplicity x s') acc) s s'.
 Definition equal (s s' : t) := M.equal Pos.eqb s s'.
 Definition subset s s' := is_empty (diff s s').
-(* Definition fold {A} f (s : t) := @M.fold _ A (fun x _ => f x) (projS1 s). *)
 Definition fold {A} f (s : t) := @M.fold positive A (fun x y => f x (Pos.to_nat y)) s.
 Definition for_all f (s : t) := M.fold (fun x n b => b && f x (Pos.to_nat n)) s true.
 Definition exists_ f (s : t) := M.fold (fun x n b => b || f x (Pos.to_nat n)) s false.
@@ -114,7 +114,7 @@ Definition partition f (s : t) :=
                                                       else (fst acc, add x (Pos.to_nat n) (snd acc))) s (empty,empty).
 Definition cardinal (s : t) := M.fold (fun _ n acc => Pos.to_nat n + acc) s 0.
 Definition size (s : t) := M.fold (fun _ _ n => S n) s 0.
-Definition elements (s : t) := List.map (fun xy => (fst xy, Pos.to_nat (snd xy))) (M.elements s).
+Definition elements (s : t) := List.map (fun xy => (fst xy, Pos.to_nat (snd xy))) (M.bindings s).
 Definition support (s : t) := M.fold (fun x _ l => cons x l) s nil.
 Definition choose (s : t) := M.fold (fun x _ _ => Some x) s None.
 
@@ -125,19 +125,22 @@ Definition For_all (P : elt -> nat -> Prop) s := forall x, In x s -> P x (multip
 Definition Exists (P : elt -> nat -> Prop) s := exists x, In x s /\ P x (multiplicity x s).
 
 Global Notation "s  [=]  t" := (eq s t) (at level 70, no associativity).
-Global Notation "s  [<=]  t" := (Subset s t) (at level 70, no associativity).
+Global Notation "s  [c=]  t" := (Subset s t) (at level 70, no associativity).
+
+Lemma eq_Meq : forall s s', s [=] s' <-> M.Equal s s'.
+Proof.
+intros s s'. unfold eq, multiplicity, M.Equal. split; intros Heq x.
++ specialize (Heq x). destruct (M.find x s), (M.find x s').
+  - apply Pos2Nat.inj in Heq. now subst.
+  - assert (Hpos := Pos2Nat.is_pos p). omega.
+  - assert (Hpos := Pos2Nat.is_pos p). omega.
+  - reflexivity.
++ now rewrite Heq.
+Qed.
 
 Instance multiplicity_compat : Proper (E.eq ==> eq ==> Logic.eq) multiplicity.
 Proof.
-intros x y Hxy s s' ?. transitivity (multiplicity x s').
-* apply H.
-* unfold multiplicity. simpl. destruct (M.find x s') eqn:Hin.
-  + apply M.find_2 in Hin. apply (M.MapsTo_1 Hxy) in Hin.
-    apply M.find_1 in Hin. now rewrite Hin.
-  + destruct (M.find y s') eqn:Hy.
-    - apply M.find_2 in Hy. apply (M.MapsTo_1 (symmetry Hxy)) in Hy.
-      apply M.find_1 in Hy. rewrite Hy in Hin. discriminate Hin.
-    - reflexivity.
+intros x y Hxy s s' Hs. rewrite eq_Meq in Hs. unfold multiplicity. now rewrite (Mfind_compat _ _ Hxy _ _ Hs).
 Qed.
 
 Global Instance eq_equiv : Equivalence eq.
@@ -153,26 +156,27 @@ Proof. unfold In. intros. apply gt_dec. Qed.
 Lemma In_MIn : forall x s, In x s <-> M.In x s.
 Proof.
 intros x s. split; intro H.
-- exists (Pos.of_nat (multiplicity x s)). apply M.find_2. unfold In, multiplicity in *.
+- exists (Pos.of_nat (multiplicity x s)). rewrite <- M.find_spec. unfold In, multiplicity in *.
   destruct (M.find x s). now rewrite Pos2Nat.id. now inversion H.
-- destruct H as [n Hn]. apply M.find_1 in Hn. unfold In, multiplicity. rewrite Hn. now apply Pos2Nat.is_pos.
+- destruct H as [n Hn]. rewrite <- M.find_spec in Hn. unfold In, multiplicity. rewrite Hn. now apply Pos2Nat.is_pos.
 Qed.
 
 Lemma Mequal_Mequivb_equiv : forall s s' : M.t positive, M.Equal s s' <-> M.Equivb Pos.eqb s s'.
 Proof.
 intros s s'. split.
 + intro Heq. split.
-  - intro x. split; intros [e Hin]; exists e; apply M.find_1 in Hin; apply M.find_2.
-    now rewrite <- Heq. now rewrite Heq.
-  - intros x e e' He He'. apply M.find_1 in He. apply M.find_1 in He'.
+  - intro x. split; intros [e Hin]; exists e.
+      now rewrite <- M.find_spec, <- Heq, M.find_spec.
+      now rewrite <- M.find_spec, Heq, M.find_spec.
+  - intros x e e' He He'. rewrite <- M.find_spec in *.
     rewrite Heq in He. rewrite He in He'. inversion_clear He'. unfold Cmp. now apply Pos.eqb_refl.
 + intros [Heq1 Heq2] x.
   destruct (M.find x s) as [e |] eqn:Hfind, (M.find x s') as [e' |] eqn:Hfind'.
-  - f_equal. apply Pos.eqb_eq. apply (Heq2 x); now apply M.find_2.
-  - assert (Habs : M.In x s'). { rewrite <- Heq1. exists e. now apply M.find_2. }
-    destruct Habs as [e' Habs]. apply M.find_1 in Habs. rewrite Hfind' in Habs. discriminate Habs.
-  - assert (Habs : M.In x s). { rewrite Heq1. exists e'. now apply M.find_2. }
-    destruct Habs as [e Habs]. apply M.find_1 in Habs. rewrite Hfind in Habs. discriminate Habs.
+  - f_equal. apply Pos.eqb_eq. apply (Heq2 x); now rewrite <- M.find_spec.
+  - assert (Habs : M.In x s'). { rewrite <- Heq1. exists e. now rewrite <- M.find_spec. }
+    destruct Habs as [e' Habs]. rewrite <- M.find_spec, Hfind' in Habs. discriminate Habs.
+  - assert (Habs : M.In x s). { rewrite Heq1. exists e'. now rewrite <- M.find_spec. }
+    destruct Habs as [e Habs]. rewrite <- M.find_spec, Hfind in Habs. discriminate Habs.
   - reflexivity.
 Qed.
 
@@ -195,11 +199,11 @@ Qed.
 Lemma equal_spec : forall s s', equal s s' = true <-> s[=]s'.
 Proof.
 intros s s'. unfold equal. simpl. destruct (M.equal Pos.eqb s s') eqn:Heq.
-+ split; intro H; trivial || clear H. apply M.equal_2 in Heq.
-  rewrite <- Mequal_Mequivb_equiv in Heq. unfold eq, multiplicity. intro. now rewrite Heq.
++ split; intro H; trivial || clear H. rewrite M.equal_spec, <- Mequal_Mequivb_equiv in Heq.
+  unfold eq, multiplicity. intro. now rewrite Heq.
 + split; intro Habs; try discriminate Habs. exfalso.
   assert (Hneq : ~M.Equivb Pos.eqb s s').
-  { intro Habs'. apply M.equal_1 in Habs'. rewrite Heq in Habs'. discriminate Habs'. }
+  { intro Habs'. rewrite <- M.equal_spec, Heq in Habs'. discriminate Habs'. }
   rewrite <- Mequal_Mequivb_equiv in Hneq. apply Hneq. intro x.
   unfold eq, multiplicity in Habs. specialize (Habs x). simpl in Habs.
   destruct (M.find x s) eqn:Hin1, (M.find x s') eqn:Hin2.
@@ -219,97 +223,68 @@ Qed.
 Lemma empty_spec : forall x, multiplicity x empty = 0.
 Proof.
 intro x. unfold multiplicity, empty.
-destruct (M.find x (M.empty positive)) eqn:Hin.
-- elim (@M.empty_1 positive x p). now apply M.find_2.
+destruct (M.find x M.empty) eqn:Hin.
+- rewrite (M.empty_spec positive x) in Hin. discriminate Hin.
 - reflexivity.
 Qed.
 
 Lemma is_empty_spec : forall s, is_empty s = true <-> s [=] empty.
 Proof.
 intros s. unfold is_empty. split; intro H.
-+ apply M.is_empty_2 in H. intros x. unfold M.Empty in H. rewrite empty_spec.
-  unfold multiplicity. destruct (M.find x s) eqn:Hin.
-  - elim (H x p). now apply M.find_2.
-  - reflexivity.
-+ apply M.is_empty_1. intros x n Habs. apply M.find_1 in Habs. specialize (H x). rewrite empty_spec in H.
-  unfold multiplicity in H. rewrite Habs in H. elim (lt_irrefl 0). rewrite <- H at 2. apply Pos2Nat.is_pos.
++ rewrite M.is_empty_spec in H. intros x. rewrite empty_spec.
+  unfold multiplicity. now rewrite H.
++ rewrite M.is_empty_spec. intro x. rewrite eq_Meq in H. rewrite H. apply M.empty_spec.
 Qed.
 
 Corollary is_empty_multiplicity : forall x s, is_empty s = true -> multiplicity x s = 0.
 Proof.
-intros x s Hs. unfold multiplicity. destruct (M.find x s) eqn:Hin.
-+ rewrite is_empty_spec in Hs. specialize (Hs x). unfold multiplicity in Hs. rewrite Hin in Hs.
-  rewrite Hs. destruct (M.find x empty) eqn:Habs.
-  - apply M.find_2 in Habs. now elim (M.empty_1 Habs).
-  - reflexivity.
-+ reflexivity.
+intros x s Hs. unfold multiplicity. destruct (M.find x s) eqn:Hin; trivial.
+rewrite is_empty_spec in Hs. rewrite eq_Meq in Hs. rewrite Hs, M.empty_spec in Hin. discriminate.
 Qed.
 
 Lemma add_same : forall x n s, multiplicity x (add x n s) = multiplicity x s + n.
 Proof.
 intros x n s. unfold add. destruct (eq_nat_dec n 0). omega.
 unfold multiplicity at 1. simpl.
-rewrite (M.find_1 (M.add_1 s (Pos.of_nat (multiplicity x s + n)) (reflexivity x))).
+rewrite (M.add_spec1 s x (Pos.of_nat (multiplicity x s + n))).
 rewrite Nat2Pos.id. reflexivity. omega.
 Qed.
 
 Lemma add_other : forall x y n s, ~E.eq y x -> multiplicity y (add x n s) = multiplicity y s.
 Proof.
-intros x y n s Hyx. unfold add. destruct (eq_nat_dec n 0). reflexivity. unfold multiplicity at 1 3. simpl.
-assert (Hxy : ~E.eq x y) by auto. destruct (M.find y s) eqn:Heq.
-+ apply (@M.add_2 positive s x y (Pos.of_nat (multiplicity y s)) (Pos.of_nat (multiplicity x s + n))) in Hxy.
-  - apply M.find_1 in Hxy. rewrite Hxy. unfold multiplicity. now rewrite Heq, Pos2Nat.id.
-  - apply M.find_2. unfold multiplicity. now rewrite Heq, Pos2Nat.id.
-+ destruct (M.find y (M.add x (Pos.of_nat (multiplicity x s + n)) s)) eqn:Heq2.
-  - apply M.find_2 in Heq2. apply (M.add_3 Hxy) in Heq2. apply M.find_1 in Heq2.
-    rewrite Heq2 in Heq. discriminate Heq.
-  - reflexivity.
+intros x y n s Hyx. unfold add. destruct (eq_nat_dec n 0); trivial. unfold multiplicity at 1 3.
+rewrite (M.add_spec2 s (Pos.of_nat (multiplicity x s + n))). reflexivity. now intro; apply Hyx.
 Qed.
 
 Lemma remove_same : forall x n s, multiplicity x (remove x n s) = multiplicity x s - n.
 Proof.
 intros x n s. unfold remove. destruct (eq_nat_dec n 0). omega.
 destruct (le_lt_dec (multiplicity x s) n) as [Hle | Hlt]; unfold multiplicity at 1; simpl.
-+ destruct (M.find x (M.remove x s)) eqn:Hin.
-  - apply M.find_2 in Hin. exfalso. apply (@M.remove_1 _ s x x (reflexivity x)). now exists p.
-  - omega.
-+ assert (Heq : M.find x (M.add x (Pos.of_nat (multiplicity x s - n)) s) = Some (Pos.of_nat (multiplicity x s - n))).
-  { apply M.find_1. apply M.add_1. reflexivity. }
-  rewrite Heq, Nat2Pos.id. reflexivity. omega.
+- rewrite M.remove_spec1. omega.
+- rewrite M.add_spec1. rewrite Nat2Pos.id. reflexivity. omega.
 Qed.
 
 Lemma remove_other : forall x y n s, ~E.eq y x -> multiplicity y (remove x n s) = multiplicity y s.
 Proof.
-intros x y n s Hyx. unfold remove. destruct (eq_nat_dec n 0). reflexivity.
-assert (Hxy : ~E.eq x y) by auto.
+intros x y n s Hyx. unfold remove. destruct (eq_nat_dec n 0); trivial.
+assert (Hxy : ~E.eq x y) by (intro; now apply Hyx).
 destruct (le_lt_dec (multiplicity x s) n) as [Hle | Hlt]; unfold multiplicity at 1; simpl.
-* destruct (M.find y (M.remove x s)) eqn:Hin.
-  + apply M.find_2, (@M.remove_3 _ s), M.find_1 in Hin. unfold multiplicity. now rewrite Hin.
-  + unfold multiplicity. destruct (M.find y s) eqn:Habs.
-    - apply M.find_2, (M.remove_2 Hxy), M.find_1 in Habs. rewrite Hin in Habs. discriminate Habs.
-    - reflexivity.
-* unfold multiplicity at 2. destruct (M.find y s) eqn:Hin.
-  + apply M.find_2, (M.add_2 (Pos.of_nat (multiplicity x s - n)) Hxy), M.find_1 in Hin. now rewrite Hin.
-  + destruct (M.find y (M.add x (Pos.of_nat (multiplicity x s - n)) s)) eqn:Habs.
-    - apply M.find_2, (@M.add_3 _ s), M.find_1 in Habs. rewrite Hin in Habs. discriminate Habs. assumption.
-    - reflexivity.
+- now rewrite M.remove_spec2.
+- now rewrite M.add_spec2.
 Qed.
 
 Lemma singleton_same : forall x n, multiplicity x (singleton x n) = n.
 Proof.
 intros x n. unfold singleton, add. destruct (eq_nat_dec n 0).
 + subst n. apply empty_spec.
-+ rewrite empty_spec. simpl. unfold multiplicity.
-  rewrite (M.find_1 (M.add_1 _ _ (reflexivity _))). now apply Nat2Pos.id.
++ rewrite empty_spec. simpl. unfold multiplicity. rewrite M.add_spec1. now apply Nat2Pos.id.
 Qed.
 
 Lemma singleton_other : forall x y n, ~E.eq y x -> multiplicity y (singleton x n) = 0.
 Proof.
 intros x y n Heq. unfold singleton, add. destruct (eq_nat_dec n 0).
 + subst n. apply empty_spec.
-+ rewrite empty_spec. simpl. unfold multiplicity.
-  destruct (M.find y (M.add x (Pos.of_nat n) empty)) eqn:Hin; trivial.
-  apply M.find_2, M.add_3 in Hin. exfalso. apply (M.empty_1 Hin). now auto.
++ rewrite empty_spec. simpl. unfold multiplicity. rewrite M.add_spec2, M.empty_spec; trivial. intro; now apply Heq.
 Qed.
 
 Lemma fold_add_out_list : forall f x n l s, ~InA (@M.eq_key positive) (x, n) l -> NoDupA (@M.eq_key _) l ->
@@ -323,10 +298,10 @@ Qed.
 Lemma fold_add_out : forall f x (s s' : t), ~M.In x s -> 
   multiplicity x (M.fold (fun x n acc => add x (f x n) acc) s s') = multiplicity x s'.
 Proof.
-intros f x s s' Hin. rewrite M.fold_1.
-assert (Hs : forall n, ~(InA (@M.eq_key_elt _) (x, n) (M.elements s))).
-{ intros n Habs. apply Hin. exists n. now apply M.elements_2. }
-revert s'. induction (M.elements s) as [| [y m] l]; intro s'; simpl.
+intros f x s s' Hin. rewrite M.fold_spec.
+assert (Hs : forall n, ~(InA (@M.eq_key_elt _) (x, n) (M.bindings s))).
+{ intros n Habs. apply Hin. exists n. now rewrite <- M.bindings_spec1. }
+revert s'. induction (M.bindings s) as [| [y m] l]; intro s'; simpl.
 + reflexivity.
 + assert ( Hxy : ~E.eq x y). { intro Habs. apply (Hs m). left. now split. }
   rewrite IHl.
@@ -340,10 +315,10 @@ Lemma fold_add : forall f x (s s' : t), compatb f -> M.In x s ->
   multiplicity x (M.fold (fun x n acc => add x (f x (Pos.to_nat n)) acc) s s')
   = f x (multiplicity x s) + multiplicity x s'.
 Proof.
-intros f x s s' Hf [n Hin]. rewrite M.fold_1.
-assert (Hs : InA (@M.eq_key_elt positive) (x, n) (M.elements s)) by now apply M.elements_1.
-assert (Hdup := M.elements_3w s).
-revert s'. induction (M.elements s) as [| [y m] l]; intro s'; simpl; [now inversion Hs |].
+intros f x s s' Hf [n Hin]. rewrite M.fold_spec.
+assert (Hs : InA (@M.eq_key_elt positive) (x, n) (M.bindings s)) by now rewrite M.bindings_spec1.
+assert (Hdup := M.bindings_spec2w s).
+revert s'. induction (M.bindings s) as [| [y m] l]; intro s'; simpl; [now inversion Hs |].
 destruct (Meq_dec (x, n) (y, m)) as [[H1 H2] | Hneq]; simpl in *; try subst m.
 * transitivity (multiplicity x (add y (f y (Pos.to_nat n)) s')).
   + rewrite (fold_add_out_list (fun x y => f x (Pos.to_nat y)) x n).
@@ -351,7 +326,7 @@ destruct (Meq_dec (x, n) (y, m)) as [[H1 H2] | Hneq]; simpl in *; try subst m.
     - inversion_clear Hdup. clear -H H1. intro Habs. apply H. revert Habs. apply InA_eqA; trivial. refine _.
     - now inversion_clear Hdup.
   + rewrite H1, add_same, plus_comm. f_equal. unfold multiplicity.
-    apply (M.MapsTo_1 H1) in Hin. apply M.find_1 in Hin. now rewrite Hin.
+    rewrite H1, <- M.find_spec in Hin. now rewrite Hin.
 * rewrite IHl.
   + f_equal. apply add_other. intro Habs. apply Hneq. compute. split. now auto.
     apply (NoDup_pair_In _ x y n m ((y, m) :: l)); trivial. left. compute. now auto.
@@ -362,9 +337,9 @@ Qed.
 Lemma union_spec : forall x s s', multiplicity x (union s s') = multiplicity x s + multiplicity x s'.
 Proof.
 intros x s s'. unfold union. destruct (M.find x s) eqn:Hin.
-- apply (fold_add (fun x n => n)). now intros until 2. exists p. now apply M.find_2.
+- apply (fold_add (fun x n => n)). now intros until 2. exists p. now rewrite <- M.find_spec.
 - unfold multiplicity at 2. rewrite Hin. simpl. apply fold_add_out.
-  intros [n Habs]. apply M.find_1 in Habs. rewrite Hin in Habs. discriminate Habs.
+  intros [n Habs]. now rewrite <- M.find_spec, Hin in Habs.
 Qed.
 
 Lemma inter_spec : forall x s s', multiplicity x (inter s s') = min (multiplicity x s) (multiplicity x s').
@@ -373,10 +348,10 @@ intros x s s'. unfold inter. destruct (M.find x s') eqn:Hin.
 + rewrite (fold_add (fun x n => min (multiplicity x s) n) x s' empty).
   - rewrite (empty_spec x). now rewrite plus_0_r.
   - intros ? ? Heq ? ? ?. simpl. subst. now rewrite Heq.
-  - exists p. now apply M.find_2.
+  - exists p. now rewrite <- M.find_spec.
 + rewrite fold_add_out.
   - unfold multiplicity at 3. rewrite Hin. rewrite Min.min_0_r. now apply empty_spec.
-  - intros [n Habs]. apply M.find_1 in Habs. rewrite Hin in Habs. discriminate Habs.
+  - intros [n Habs]. now rewrite <- M.find_spec, Hin in Habs.
 Qed.
 
 Lemma diff_spec : forall x s s', multiplicity x (diff s s') = multiplicity x s - multiplicity x s'.
@@ -385,10 +360,10 @@ intros x s s'. unfold diff. destruct (M.find x s) eqn:Hin.
 + rewrite (fold_add (fun x n => n - multiplicity x s') x s empty).
   - rewrite empty_spec. now rewrite plus_0_r.
   - intros ? ? Heq ? ? ?. subst. now rewrite Heq.
-  - exists p. now apply M.find_2.
+  - exists p. now rewrite <- M.find_spec.
 + rewrite fold_add_out.
   - unfold multiplicity at 2. rewrite Hin. simpl. now apply empty_spec.
-  - intros [n Habs]. apply M.find_1 in Habs. rewrite Hin in Habs. discriminate Habs.
+  - intros [n Habs]. now rewrite <- M.find_spec, Hin in Habs.
 Qed.
 
 Lemma lub_spec : forall x s s', multiplicity x (lub s s') = max (multiplicity x s) (multiplicity x s').
@@ -400,45 +375,43 @@ replace (max (multiplicity x s) (multiplicity x s'))
 destruct (M.find x s) eqn:Hin.
 + apply (fold_add (fun x n => n - multiplicity x s')).
   - intros ? ? Heq ? ? ?. subst. now rewrite Heq.
-  - exists p. now apply M.find_2.
+  - exists p. now rewrite <- M.find_spec.
 + rewrite fold_add_out.
   - unfold multiplicity at 2. rewrite Hin. simpl. reflexivity.
-  - intros [n Habs]. apply M.find_1 in Habs. rewrite Hin in Habs. discriminate Habs.
+  - intros [n Habs]. now rewrite <- M.find_spec, Hin in Habs.
 Qed.
 
-Lemma subset_spec : forall s s', subset s s' = true <-> s [<=] s'.
+Lemma subset_spec : forall s s', subset s s' = true <-> s [c=] s'.
 Proof.
 intros s s'. split; intro Hle.
 - intro x. apply (is_empty_multiplicity x) in Hle. rewrite diff_spec in Hle. omega.
 - unfold subset. rewrite is_empty_spec. intro x. unfold In. rewrite diff_spec.
   specialize (Hle x). rewrite empty_spec. omega.
 Qed.
-(*
-Lemma fold_spec : forall (A : Type) (i : A) (f : elt -> A -> A) s,
-    fold f s i = fold_left (flip f) (elements s) i.
-*)
+
 Lemma fold_spec : forall (A : Type) s (i : A) (f : elt -> nat -> A -> A),
     fold f s i = fold_left (fun acc xn => f (fst xn) (snd xn) acc) (elements s) i.
-Proof. intros A i f s. unfold fold, elements. now rewrite M.fold_1, fold_left_map. Qed.
+Proof. intros A i f s. unfold fold, elements. now rewrite M.fold_spec, fold_left_map. Qed.
 
 Lemma cardinal_spec : forall s, cardinal s = fold (fun x n acc => n + acc) s 0.
-Proof. intro. unfold cardinal. rewrite fold_spec. unfold elements. now rewrite fold_left_map, M.fold_1. Qed.
+Proof. intro. unfold cardinal. rewrite fold_spec. unfold elements. now rewrite fold_left_map, M.fold_spec. Qed.
 
 Lemma size_spec : forall s, size s = length (support s).
-Proof. intro. unfold size, support. now rewrite M.fold_1, fold_left_length, M.fold_1, fold_left_cons_length. Qed.
+Proof.
+intro. unfold size, support. now rewrite M.fold_spec, fold_left_length, M.fold_spec, fold_left_cons_length.
+Qed.
 
 
 Lemma Melements_multiplicity : forall s x n,
-  InA (@M.eq_key_elt _) (x, n) (M.elements s)
+  InA (@M.eq_key_elt _) (x, n) (M.bindings s)
   <-> multiplicity x s = Pos.to_nat n /\ Pos.to_nat n > 0.
 Proof.
-intros s x n. simpl.
-split; intro H.
-+ apply M.elements_2 in H. apply M.find_1 in H. unfold multiplicity. 
+intros s x n. split; intro H.
++ apply M.bindings_spec1, M.find_spec in H. unfold multiplicity.
   rewrite H. split. reflexivity. apply Pos2Nat.is_pos.
 + destruct H as [H1 H2]. unfold multiplicity in H1. destruct (M.find x s) eqn:Hin.
-  - apply M.elements_1. apply M.find_2. rewrite Hin. f_equal. now apply Pos2Nat.inj.
-  - rewrite  <-H1 in H2. inversion H2.
+  - rewrite M.bindings_spec1, <- M.find_spec. rewrite Hin. f_equal. now apply Pos2Nat.inj.
+  - rewrite  <- H1 in H2. inversion H2.
 Qed.
 
 Corollary elements_spec : forall x n s,
@@ -459,7 +432,7 @@ Qed.
 Lemma elements_NoDupA : forall s, NoDupA (@M.eq_key _) (elements s).
 Proof.
 intro s. unfold elements. rewrite NoDupA_inj_map; 
-apply M.elements_3w || apply Meq_key_equiv || (intros [] [] ?; assumption).
+apply M.bindings_spec2w || apply Meq_key_equiv || (intros [] [] ?; assumption).
 Qed.
 
 Lemma support_elements_aux : forall x l1 l2, NoDupA (@M.eq_key _) (l1 ++ l2) -> 
@@ -498,9 +471,9 @@ Qed.
 
 Lemma support_elements : forall x s, InA E.eq x (support s) <-> InA eq_pair (x, multiplicity x s) (elements s).
 Proof.
-intros x s. unfold support, elements. rewrite M.fold_1.
+intros x s. unfold support, elements. rewrite M.fold_spec.
 change nil with (map (@fst E.t nat) nil).
-rewrite (support_elements_aux x (M.elements s) nil); rewrite app_nil_r; [split; intro H |].
+rewrite (support_elements_aux x (M.bindings s) nil); rewrite app_nil_r; [split; intro H |].
 + destruct H as [n Hn].
   assert (n = multiplicity x s).
   { rewrite (InA_map_iff (Meq_equiv _) eq_pair_equiv) in Hn.
@@ -509,7 +482,7 @@ rewrite (support_elements_aux x (M.elements s) nil); rewrite app_nil_r; [split; 
     - intros [? ?] [? ?] Heq; simpl in *. hnf in Heq. destruct Heq; split; hnf; simpl in *; subst; auto. }
   now subst n.
 + now exists (multiplicity x s).
-+ apply M.elements_3w.
++ apply M.bindings_spec2w.
 Qed.
 
 Corollary support_spec : forall x s, InA E.eq x (support s) <-> In x s.
@@ -525,9 +498,9 @@ Qed.
 
 Lemma support_NoDupA : forall s, NoDupA E.eq (support s).
 Proof.
-intro s. unfold support. rewrite M.fold_1. rewrite support_NoDupA_aux. rewrite app_nil_r.
+intro s. unfold support. rewrite M.fold_spec, support_NoDupA_aux, app_nil_r.
 apply NoDupA_rev. now auto with typeclass_instances.
-rewrite NoDupA_inj_map; (now apply M.elements_3w) || (now auto with typeclass_instances) || (now intros ? ? ?).
+rewrite NoDupA_inj_map; (now apply M.bindings_spec2w) || (now auto with typeclass_instances) || (now intros ? ? ?).
 Qed.
 
 
@@ -551,11 +524,11 @@ Lemma filter_spec_In : forall f s s' x, compatb f -> In x s ->
         if f x0 (Pos.to_nat n) : bool then add x0 (Pos.to_nat n) acc else acc) s s')
   = if f x (multiplicity x s) then multiplicity x s + multiplicity x s' else multiplicity x s'.
 Proof.
-intros f s s' x Hf Hin. rewrite M.fold_1. revert s'. unfold In in Hin.
+intros f s s' x Hf Hin. rewrite M.fold_spec. revert s'. unfold In in Hin.
 assert (Hs : InA (@M.eq_key_elt _) (x, multiplicity x s) (elements s)). { rewrite elements_spec. simpl. now split. }
 assert (Hdup : NoDupA (@M.eq_key _) (elements s)) by apply elements_NoDupA.
 unfold elements in Hs, Hdup.
-induction (M.elements s); simpl; intro s'; simpl in Hs.
+induction (M.bindings s); simpl; intro s'; simpl in Hs.
 * exfalso. rewrite <- InA_nil. apply Hs.
 * destruct a as [y m].
   destruct (Meq_dec (x, Pos.of_nat (multiplicity x s)) (y, m)) as [Heq | Hneq].
@@ -592,11 +565,11 @@ Lemma filter_spec_out : forall f s s' x, ~In x s ->
         if f x0 (Pos.to_nat n) : bool then add x0 (Pos.to_nat n) acc else acc) s s')
   = multiplicity x s'.
 Proof.
-intros f s s' x Hin. rewrite M.fold_1.
-assert (Hs : forall n, ~(InA (@M.eq_key_elt _) (x, n) (M.elements s))).
-{ intros n Habs. apply Hin. apply M.elements_2 in Habs. apply M.find_1 in Habs.
+intros f s s' x Hin. rewrite M.fold_spec.
+assert (Hs : forall n, ~(InA (@M.eq_key_elt _) (x, n) (M.bindings s))).
+{ intros n Habs. apply Hin. rewrite M.bindings_spec1, <- M.find_spec in Habs.
   unfold In, multiplicity. rewrite Habs. apply Pos2Nat.is_pos. }
-revert s'. induction (M.elements s) as [| [y m] l]; intro s'; simpl.
+revert s'. induction (M.bindings s) as [| [y m] l]; intro s'; simpl.
   reflexivity.
   assert ( Hxy : ~E.eq x y). { intro Habs. apply (Hs m). left. now split. }
   rewrite IHl. destruct (f y (Pos.to_nat m)). apply add_other. now auto. reflexivity.
@@ -619,31 +592,31 @@ Qed.
 
 
 Lemma choose_spec_aux : forall x s o, ~M.In x s ->
-  fold_left (fun (_ : option M.key) (p : M.key * positive) => Some (fst p)) (M.elements s) o = Some x ->
+  fold_left (fun (_ : option M.key) (p : M.key * positive) => Some (fst p)) (M.bindings s) o = Some x ->
   o = Some x.
 Proof.
 intros x s o Hs.
-assert (Hs' : forall n, ~InA (@M.eq_key_elt _) (x, n) (M.elements s)).
-{ intros n Habs. apply Hs. exists n. now apply M.elements_2. } clear Hs.
-revert o. induction (M.elements s); simpl; intros o Hin.
-  assumption.
-  apply IHl in Hin.
-    elim (Hs' (snd a)). left. split; simpl. now inversion Hin. reflexivity.
-    intros n Habs. apply (Hs' n). now right.
+assert (Hs' : forall n, ~InA (@M.eq_key_elt _) (x, n) (M.bindings s)).
+{ intros n Habs. apply Hs. exists n. now apply M.bindings_spec1. } clear Hs.
+revert o. induction (M.bindings s); simpl; intros o Hin.
++ assumption.
++ apply IHl in Hin.
+  - elim (Hs' (snd a)). left. split; simpl. now inversion Hin. reflexivity.
+  - intros n Habs. apply (Hs' n). now right.
 Qed.
 
 Lemma choose_Some : forall x s, choose s = Some x -> In x s.
 Proof.
 intros x s Hin. destruct (In_dec x s). assumption. unfold choose in Hin.
-rewrite M.fold_1 in Hin. apply choose_spec_aux in Hin. now inversion Hin. now rewrite <- In_MIn.
+rewrite M.fold_spec in Hin. apply choose_spec_aux in Hin. now inversion Hin. now rewrite <- In_MIn.
 Qed.
 
 Lemma choose_None : forall s, choose s = None <-> s [=] empty.
 Proof.
 intros s. split; intro Hs.
-+ intro x. unfold choose in Hs. rewrite M.fold_1 in Hs. rewrite empty_spec, multiplicity_out.
++ intro x. unfold choose in Hs. rewrite M.fold_spec in Hs. rewrite empty_spec, multiplicity_out.
   destruct (M.find x s) eqn:Habs.
-  - apply M.find_2 in Habs. apply M.elements_1 in Habs. destruct (M.elements s).
+  - rewrite M.find_spec, <- M.bindings_spec1 in Habs. destruct (M.bindings s).
       now inversion Habs.
       clear -Hs. simpl in Hs. revert p0 Hs. induction l. discriminate. intros. simpl in Hs. now apply (IHl _ Hs).
   - reflexivity.
@@ -656,8 +629,8 @@ Lemma fold_and_true_base_step : forall A f (l : list A) b,
   fold_left (fun a x => a && f x) l b = true -> b = true.
 Proof.
 intros A f l. induction l; simpl; intros b Hl.
-  assumption.
-  apply IHl in Hl. destruct b. reflexivity. simpl in Hl. discriminate Hl.
+- assumption.
+- apply IHl in Hl. destruct b. reflexivity. simpl in Hl. discriminate Hl.
 Qed.
 
 Lemma fold_and_true_inductive_step : forall A f (l : list A) a b, 
@@ -671,19 +644,19 @@ Lemma for_all_spec_aux : forall (f : M.key -> nat -> bool) s b, compatb f ->
   (M.fold (fun x n b => b && (f x (Pos.to_nat n))) s b = true
    <-> b = true /\ For_all (fun x n => f x n = true) s).
 Proof.
-intros f s b Hf. rewrite M.fold_1. unfold For_all. split; intro H.
+intros f s b Hf. rewrite M.fold_spec. unfold For_all. split; intro H.
 + split. now apply fold_and_true_base_step in H.
-  intros x Hin. rewrite In_MIn in Hin. destruct Hin as [n Hin]. apply M.elements_1 in Hin.
+  intros x Hin. rewrite In_MIn in Hin. destruct Hin as [n Hin]. apply M.bindings_spec1 in Hin.
   assert (Hn : multiplicity x s = Pos.to_nat n) by now rewrite Melements_multiplicity in Hin.
-  revert b H x n Hn Hin. induction (M.elements s); intros b H x n Hn Hin; inversion_clear Hin.
+  revert b H x n Hn Hin. induction (M.bindings s); intros b H x n Hn Hin; inversion_clear Hin.
   - simpl in H. apply fold_and_true_base_step in H. rewrite andb_true_iff in H.
     destruct H as [_ H ], a, H0 as [H1 H2]. simpl in *. rewrite Hn, H1. now subst p.
   - simpl in H. apply (IHl _ H _ _ Hn H0).
 + destruct H as [Hb H]. subst b.
-  assert (forall xn, InA (@M.eq_key_elt _) xn (M.elements s) -> f (fst xn) (Pos.to_nat (snd xn)) = true).
+  assert (forall xn, InA (@M.eq_key_elt _) xn (M.bindings s) -> f (fst xn) (Pos.to_nat (snd xn)) = true).
   { intros [x n] Hx. simpl. rewrite Melements_multiplicity in Hx. destruct Hx as [Hm Hp].
     setoid_rewrite <- Pos2Nat.id. rewrite <- Hm. rewrite Nat2Pos.id. apply H. unfold In. now rewrite Hm. omega. }
-  clear H. revert H0. induction (M.elements s); simpl; intro Hin; trivial.
+  clear H. revert H0. induction (M.bindings s); simpl; intro Hin; trivial.
   rewrite Hin. apply IHl. intros x Hx. apply Hin. now right. now left.
 Qed.
 
@@ -697,7 +670,7 @@ Lemma exists_spec_aux : forall (f : M.key -> nat -> bool) s b, compatb f ->
 Proof.
 intros f s b Hf.
 assert (Hequiv : Exists (fun x n => f x n = true) s <->
-        exists x, exists n, InA (@M.eq_key_elt _) (x, n) (M.elements s) /\ f x (Pos.to_nat n) = true).
+        exists x, exists n, InA (@M.eq_key_elt _) (x, n) (M.bindings s) /\ f x (Pos.to_nat n) = true).
 { split; intros [x Hx].
   destruct Hx as [Hin Hfx]. exists x. exists (Pos.of_nat (multiplicity x s)). split.
     rewrite Melements_multiplicity. unfold In in Hin. simpl. rewrite Nat2Pos.id. now split. omega.
@@ -705,13 +678,13 @@ assert (Hequiv : Exists (fun x n => f x n = true) s <->
   destruct Hx as [n [Hin Hfx]]. exists x. rewrite Melements_multiplicity in Hin. destruct Hin as [Hn Hp]. split.
     simpl in *. unfold In. now rewrite Hn.
     simpl in *. now rewrite Hn. }
-rewrite Hequiv. clear Hequiv. rewrite M.fold_1. unfold For_all. split; intro H.
-+ revert b H. induction (M.elements s); intros b H.
+rewrite Hequiv. clear Hequiv. rewrite M.fold_spec. unfold For_all. split; intro H.
++ revert b H. induction (M.bindings s); intros b H.
   - simpl in H. now left.
   - simpl in H. apply IHl in H. rewrite orb_true_iff in H. destruct H as [[H | H] | H]; (now left) || right.
       destruct a as [x n]. exists x. exists n. split. now left. assumption.
       destruct H as [x [n [Hin Hfx]]]. exists x. exists n. split. now right. assumption.  
-+ revert b H. induction (M.elements s); simpl; intros b H.
++ revert b H. induction (M.bindings s); simpl; intros b H.
   - destruct H. assumption.
     destruct H as [? [? [Habs _]]]. now inversion Habs.
   - apply IHl. rewrite orb_true_iff. destruct H as [H | H].
@@ -756,11 +729,11 @@ Lemma partition_spec_fst_In : forall f (s : t) (s12 : t * t) x, compatb f -> In 
          else (fst acc, add x (Pos.to_nat n) (snd acc))) s s12)) =
   (if f x (multiplicity x s) then multiplicity x s + multiplicity x (fst s12) else multiplicity x (fst s12)).
 Proof.
-intros f s s' x Hf Hin. rewrite M.fold_1. revert s'. unfold In in Hin.
+intros f s s' x Hf Hin. rewrite M.fold_spec. revert s'. unfold In in Hin.
 assert (Hs : InA (@M.eq_key_elt _) (x, multiplicity x s) (elements s)). { rewrite elements_spec. simpl. now split. }
 assert (Hdup : NoDupA (@M.eq_key _) (elements s)) by apply elements_NoDupA.
 unfold elements in Hs, Hdup.
-induction (M.elements s); simpl; intros [s1 s2]; simpl in Hs.
+induction (M.bindings s); simpl; intros [s1 s2]; simpl in Hs.
 * exfalso. rewrite <- InA_nil. apply Hs.
 * destruct a as [y m].
   destruct (Meq_dec (x, Pos.of_nat (multiplicity x s)) (y, m)) as [Heq | Hneq].
@@ -796,11 +769,11 @@ Lemma partition_spec_fst_out : forall f s s12 x, ~In x s ->
          then (add x (Pos.to_nat n) (fst acc), snd acc)
          else (fst acc, add x (Pos.to_nat n) (snd acc))) s s12)) = multiplicity x (fst s12).
 Proof.
-intros f s s' x Hin. rewrite M.fold_1.
-assert (Hs : forall n, ~(InA (@M.eq_key_elt _) (x, n) (M.elements s))).
-{ intros n Habs. apply Hin. apply M.elements_2 in Habs. apply M.find_1 in Habs.
+intros f s s' x Hin. rewrite M.fold_spec.
+assert (Hs : forall n, ~(InA (@M.eq_key_elt _) (x, n) (M.bindings s))).
+{ intros n Habs. apply Hin. rewrite M.bindings_spec1, <- M.find_spec in Habs.
   unfold In, multiplicity. rewrite Habs. apply Pos2Nat.is_pos. }
-revert s'. induction (M.elements s) as [| [y m] l]; intro s'; simpl.
+revert s'. induction (M.bindings s) as [| [y m] l]; intro s'; simpl.
   reflexivity.
   assert ( Hxy : ~E.eq x y). { intro Habs. apply (Hs m). left. now split. }
   rewrite IHl. unfold partition_fun. destruct (f y (Pos.to_nat m)). apply add_other. now auto. reflexivity.
@@ -849,11 +822,11 @@ Lemma partition_spec_snd_In : forall f (s : t) (s12 : t * t) x, compatb f -> In 
          else (fst acc, add y (Pos.to_nat n) (snd acc))) s s12)) =
   (if f x (multiplicity x s) then multiplicity x (snd s12) else multiplicity x s + multiplicity x (snd s12)).
 Proof.
-intros f s s' x Hf Hin. rewrite M.fold_1. revert s'. unfold In in Hin.
+intros f s s' x Hf Hin. rewrite M.fold_spec. revert s'. unfold In in Hin.
 assert (Hs : InA (@M.eq_key_elt _) (x, multiplicity x s) (elements s)). { rewrite elements_spec. simpl. now split. }
 assert (Hdup : NoDupA (@M.eq_key _) (elements s)) by apply elements_NoDupA.
 unfold elements in Hs, Hdup.
-induction (M.elements s); simpl; intros [s1 s2]; simpl in Hs.
+induction (M.bindings s); simpl; intros [s1 s2]; simpl in Hs.
 * exfalso. rewrite <- InA_nil. apply Hs.
 * destruct a as [y m].
   destruct (Meq_dec (x, Pos.of_nat (multiplicity x s)) (y, m)) as [Heq | Hneq].
@@ -893,11 +866,11 @@ Lemma partition_spec_snd_out : forall f s s12 x, ~In x s ->
          else (fst acc, add y (Pos.to_nat n) (snd acc))) s s12)) =
   multiplicity x (snd s12).
 Proof.
-intros f s s' x Hin. rewrite M.fold_1.
-assert (Hs : forall n, ~(InA (@M.eq_key_elt _) (x, n) (M.elements s))).
-{ intros n Habs. apply Hin. apply M.elements_2 in Habs. apply M.find_1 in Habs.
+intros f s s' x Hin. rewrite M.fold_spec.
+assert (Hs : forall n, ~(InA (@M.eq_key_elt _) (x, n) (M.bindings s))).
+{ intros n Habs. apply Hin. rewrite M.bindings_spec1, <- M.find_spec in Habs.
   unfold In, multiplicity. rewrite Habs. apply Pos2Nat.is_pos. }
-revert s'. induction (M.elements s) as [| [y m] l]; intro s'; simpl.
+revert s'. induction (M.bindings s) as [| [y m] l]; intro s'; simpl.
   reflexivity.
   assert ( Hxy : ~E.eq x y). { intro Habs. apply (Hs m). left. now split. }
   rewrite IHl. destruct (f y (Pos.to_nat m)); simpl. reflexivity. apply add_other. now auto.
@@ -922,7 +895,7 @@ Instance fold_compat A (eqA : A -> A -> Prop) `{Equivalence A eqA} : forall f,
   Proper (E.eq ==> Logic.eq ==> eqA ==> eqA) f -> transpose2 eqA f ->
   Proper (eq ==> eqA ==> eqA) (fold f).
 Proof.
-intros f Hf Hfcomm s1 s2 Hs x y Hxy. unfold fold. do 2 rewrite M.fold_1.
+intros f Hf Hfcomm s1 s2 Hs x y Hxy. unfold fold. do 2 rewrite M.fold_spec.
 rewrite fold_left_symmetry_PermutationA.
 + reflexivity.
 + now apply Meq_equiv.
@@ -931,8 +904,8 @@ rewrite fold_left_symmetry_PermutationA.
 + intros. apply Hfcomm.
 + apply NoDupA_equivlistA_PermutationA.
   - now apply Meq_equiv.
-  - eapply NoDupA_strengthen; try apply M.elements_3w. now intros [? ?] [? ?] [? ?].
-  - eapply NoDupA_strengthen; try apply M.elements_3w. now intros [? ?] [? ?] [? ?].
+  - eapply NoDupA_strengthen; try apply M.bindings_spec2w. now intros [? ?] [? ?] [? ?].
+  - eapply NoDupA_strengthen; try apply M.bindings_spec2w. now intros [? ?] [? ?] [? ?].
   - clear -Hs. intros [x n]. do 2 rewrite Melements_multiplicity. now rewrite Hs.
 + assumption.
 Qed.
